theories/sprop.v
@@ -2,17 +2,15 @@ From Coq Require Export Logic.StrictProp.
 From stdpp Require Import decidable.
 From stdpp Require Import options.
 
-Definition SIs_true (b: bool): SProp := if b then sUnit else sEmpty.
+Lemma unsquash (P : Prop) `{!Decision P} : Squash P → P.
+Proof.
+  intros HP. destruct (decide P) as [?|HnotP]; [assumption|].
+  assert sEmpty as []. destruct HP. destruct HnotP; assumption.
+Qed.
 
-Lemma SIs_true_intro {b: bool} : Is_true b → SIs_true b.
-Proof. destruct b; [constructor | intros []]. Qed.
-Lemma SIs_true_elim {b: bool} : SIs_true b → Is_true b.
-Proof. destruct b; simpl; [constructor | intros []]. Qed.
+Definition SIs_true (b : bool) : SProp := Squash (Is_true b).
 
-Definition sprop_decide (P : Prop) `{!Decision P} : SProp :=
-  SIs_true (bool_decide P).
-
-Lemma sprop_decide_pack (P : Prop) `{!Decision P} : P → sprop_decide P.
-Proof. intros HP. apply SIs_true_intro, bool_decide_pack, HP. Qed.
-Lemma sprop_decide_unpack (P : Prop) `{!Decision P} : sprop_decide P → P.
-Proof. intros HP. apply (bool_decide_unpack P), SIs_true_elim, HP. Qed.
+Lemma SIs_true_intro b : Is_true b → SIs_true b.
+Proof. apply squash. Qed.
+Lemma SIs_true_elim b : SIs_true b → Is_true b.
+Proof. apply (unsquash _). Qed.
